src/PlutusIR/Semantics/Static/normaliser_STLC/STLC_norm_completeness.v
@@ -1,0 +1,155 @@
+From PlutusCert Require Import STLC_named STLC_normalisation SN_STLC_named STLC_named_typing util.
+Require Import Coq.Lists.List.
+Import ListNotations.
+
+Require Import Coq.Program.Equality.
+
+Lemma normalise_extend T1 T2 T3 :
+  step_d T1 T2 -> normalise T2 T3 -> normalise T1 T3.
+Proof.
+  intros Hstep Hnorm.
+  generalize dependent T3.
+  induction Hstep; intros T3 Hnorm; try solve [inversion Hnorm; try constructor; eauto].
+  eapply N_BetaReduce; eauto.
+  + apply N_TyLam.
+    admit (* Follows from normalisation__stable'__normal *).
+  + admit.  (* Follows from normalisation__stable'__normal *)
+Admitted.
+
+(* Wouter's suggestion: do not use explicit normalizer in soundness proof*)
+Theorem SN_d__normalise t :
+  SN_d t -> {t' & normalise t t'}.
+Proof.
+  intros HSN.
+  induction HSN as [t].
+  (* Suppose step_d_f t = None, then t normal, then t' = t and normalise t t *)
+  assert ({t' & step_d t t'}) as [t' Ht_steps] by admit.
+  specialize (H t' Ht_steps) as [tn normt'].
+  exists tn.
+  now apply normalise_extend with (T2 := t').
+Admitted.
+
+Definition normaliser t Δ T (Hwt : SN_STLC_named.has_type Δ t T) :=
+  let snt := strong_normalization_d Hwt in
+  projT1 (SN_d__normalise t snt).
+
+Theorem norm_sound t tn Δ T (Hwt : SN_STLC_named.has_type Δ t T) :
+  normaliser t Δ T Hwt = tn -> normalise t tn.
+Proof.
+  intros.
+  unfold normaliser in H.
+  destruct SN_d__normalise in H.
+  subst.
+  assumption.
+Qed.
+
+(* see normalisation__deterministic in Normalisation.v*)
+Lemma normalise_unique t tn1 tn2 :
+  normalise t tn1 -> normalise t tn2 -> tn1 = tn2.
+Proof.
+Admitted.
+
+Theorem norm_complete Δ K (t tn : term) (Hwt : SN_STLC_named.has_type Δ t K):
+  normalise t tn -> normaliser t Δ K Hwt = tn.
+Proof.
+  intros HnormR.
+  unfold normaliser.
+  destruct SN_d__normalise.
+  simpl.
+  now apply (normalise_unique t x tn) in n.
+Qed.
+
+(* Lemma normalise_unique_step t t' tn1 tn2 :
+  step_d_f t = Some t' -> normalise t tn1 -> normalise t' tn2 -> tn1 = tn2.
+Proof.
+  intros Hstep Hnorm1 Hnorm2.
+  assert (step_d t t') by admit.
+  generalize dependent tn2.
+  generalize dependent tn1.
+  induction H; intros tn1 Hnorm1 tn2 Hnorm2.
+  - eapply N_BetaReduce in Hnorm2; eauto. 
+    + eapply (normalise_unique); eauto.
+    + (* ?K = A and itis al l normal so yes *) admit.
+    + (* t is normal, so yes.*) admit.
+  - admit.
+  - admit.
+  - assert (step_d_f s1 = Some s2) by admit.
+    specialize (IHstep_d H0).
+    inversion Hnorm1; subst.
+    inversion Hnorm2; subst.
+    f_equal.
+    apply IHstep_d with (tn1 := T0n) (tn2 := T0n0); eauto.
+    
+Admitted. *)
+
+(* Lemma extend_normalizer7 t1 t2 s (Hstep : step_d_f t1 = Some t2) :
+  @normalizer7' t1 (SNI5 (x := t1) s) =
+  @normalizer7' t2 (s t2 Hstep).
+Proof.
+    unfold normalizer7'.
+    destruct norm_wouter.
+    destruct norm_wouter.
+    assert (x = x0).
+    {
+      apply (normalise_unique_step t1 t2 x x0 Hstep n n0).
+    }
+    subst.
+    simpl.
+    reflexivity.
+Qed.
+
+Lemma norm_lam7 tb x T (snt : (SN5 (tmlam x T tb))) (sntb : SN5 tb):
+  @normalizer7' (tmlam x T tb) snt = tmlam x T (@normalizer7' tb sntb).
+Proof.
+  intros.
+  unfold normalizer7'.
+  destruct norm_wouter.
+  simpl.
+  inversion n.
+  subst.
+  f_equal.
+  destruct norm_wouter.
+  simpl.
+  now apply (normalise_unique tb T0n x0 H3) in n0.
+Qed.
+
+(* Needs a neutrality requirement *)
+Lemma norm_app7 t1 t2 (snt : (SN5 (tmapp t1 t2))) (snt1 : SN5 t1) (snt2 : SN5 t2) :
+  STLC_normalisation.neutral_Ty (@normalizer7' t1 snt1) -> @normalizer7' (tmapp t1 t2) snt = tmapp (@normalizer7' t1 snt1) (@normalizer7' t2 snt2).
+Proof.
+Admitted. *)
+
+(* Looks complicated, but it is really a step forward, since there is no mention of normalise anymore
+  If it is too difficult, we can first try to do it with t1 already normalized fully I think.
+*)
+(* Lemma norm_subst7 t1 t2 T1n bX K1 tn (snt : (SN5 (tmapp t1 t2))) (snt1 : (SN5 t1)) (snt2 : (SN5 t2)) 
+    (snsub : (SN5 (substituteTCA bX (@normalizer7' t2 snt2) T1n))) :
+  @normalizer7' t1 snt1 = tmlam bX K1 T1n -> 
+    @normalizer7' (tmapp t1 t2) snt = tn
+    ->
+    @normalizer7' (substituteTCA bX (@normalizer7' t2 snt2) T1n) snsub = tn.
+Proof.
+  intros Hnorm1 Hnormapp.
+  simpl.
+  unfold normalizer7' in Hnormapp.
+  destruct norm_wouter in Hnormapp.
+  rewrite <- Hnormapp. clear Hnormapp.
+  unfold normalizer7' in Hnorm1.
+  destruct norm_wouter in Hnorm1.
+  simpl in Hnorm1.
+  simpl.
+  subst.
+  remember (normalizer7' t2 snt2) as prrr.
+  unfold normalizer7'.
+  destruct norm_wouter.
+  simpl.
+  eapply N_BetaReduce in n1; eauto.
+  - eapply (normalise_unique (tmapp t1 t2)); eauto.
+  - subst.
+    unfold normalizer7'.
+    destruct norm_wouter.
+    simpl.
+    assumption.
+Qed. *)
+
+
